purged one definition

Polylean/GroupRing.lean
@@ -9,158 +9,88 @@ variable (R : Type) [Ring R] [DecidableEq R]
 variable (G: Type) [Group G] [DecidableEq G]
 
 
-section direct
-
-def FormalSum.mulTerm (a: R)(g: G) : FormalSum R G → FormalSum R G 
+def FormalSum.mulTerm (b: R)(h: G) : FormalSum R G → FormalSum R G 
 | [] => []
-| (b, h) :: tail => (a * b, g * h) :: (mulTerm a g tail)
+| (a, g) :: tail => (a * b, g * h) :: (mulTerm b h tail)
 
-def FormalSum.mul: FormalSum R G → FormalSum R G → FormalSum R G
-| [] =>  fun _ =>  []
-| (a, g) :: xs => fun t => 
-  (FormalSum.mulTerm R G a g t) ++ (mul xs t)
+def FormalSum.mul(fst: FormalSum R G) : FormalSum R G → FormalSum R G
+| [] =>    []
+| (b, h) :: ys =>  
+  (FormalSum.mulTerm R G b h fst) ++ (mul fst ys)
 
-open ElementaryMove
 open FormalSum
+
+theorem mulTerm_zero (g x₀: G)(s: FormalSum R G):
+  coords (mulTerm R G 0 g s) x₀ = 0 := by
+  induction s with
+  | nil =>  
+    simp [mulTerm, coords]
+  | cons h t ih => 
+    simp [mulTerm, coords, monom_coords_at_zero]
+    assumption
 
 theorem mul_zero_cons (s t : FormalSum R G)(g: G): 
     mul R G s ((0, h) :: t) ≈  mul R G s t := by
-      induction s
-      case nil => 
-        simp [mul]
-        apply eqlCoords.refl
-      case cons head tail ih => 
-      let (a, g) := head
-      rw [mul]
-      simp
-      apply append_equiv
-      rw [mulTerm, mul_zero]
-      apply funext
-      intro x₀
-      simp [coords]
-      rw [monom_coords_at_zero]
-      rw [zero_add]
-      exact ih
-      
-
-def mulAux : FormalSum R G → FreeModule R G → FreeModule R G := by
-  intro s
-  let f  := fun t => ⟦ FormalSum.mul R G s t ⟧ 
-  apply  Quotient.lift f
-  apply func_eql_of_move_equiv
-  intro t t' rel
-  simp 
-  induction rel with
-  | zeroCoeff tail g a hyp =>
-    rw [hyp]
-    simp [mul, mulTerm]
-    apply Quotient.sound
-    apply mul_zero_cons
-    exact g
-  | addCoeffs a b x tail =>
-    apply Quotient.sound
-    cases s
-    simp [mul]
-    apply eqlCoords.refl
-    simp [mul, mulTerm]
-    apply funext
-    intro x₀
-    simp [coords]
-    simp
-    admit
-  | cons a x s₁ s₂ r step =>
-    admit
-  | swap a₁ a₂ x₁ x₂ tail =>
-    admit
-
-end direct
-
-section flipped
-
-def FormalSum.mulTerm' (b: R)(h: G) : FormalSum R G → FormalSum R G 
-| [] => []
-| (a, g) :: tail => (a * b, g * h) :: (mulTerm' b h tail)
-
-def FormalSum.mul'(fst: FormalSum R G) : FormalSum R G → FormalSum R G
-| [] =>    []
-| (b, h) :: ys =>  
-  (FormalSum.mulTerm' R G b h fst) ++ (mul' fst ys)
-
-open FormalSum
-
-theorem mulTerm_zero' (g x₀: G)(s: FormalSum R G):
-  coords (mulTerm' R G 0 g s) x₀ = 0 := by
-  induction s with
-  | nil =>  
-    simp [mulTerm', coords]
-  | cons h t ih => 
-    simp [mulTerm', coords, monom_coords_at_zero]
-    assumption
-
-theorem mul_zero_cons' (s t : FormalSum R G)(g: G): 
-    mul' R G s ((0, h) :: t) ≈  mul' R G s t := by
     induction s
     case nil =>
-      simp [mul', mulTerm']
+      simp [mul, mulTerm]
       apply eqlCoords.refl
     case cons head tail ih =>
-      simp [mul', mulTerm']
+      simp [mul, mulTerm]
       apply funext ; intro x₀
       simp [coords]
       rw [monom_coords_at_zero]
       rw [zero_add]
       rw [← append_coords]
-      simp [coords, mul']
-      let l := mulTerm_zero' R G h x₀ tail
+      simp [coords, mul]
+      let l := mulTerm_zero R G h x₀ tail
       rw [l]
       simp [zero_add]
   
-def mulAux' : FormalSum R G → FreeModule R G → FreeModule R G := by
+def mulAux : FormalSum R G → FreeModule R G → FreeModule R G := by
   intro s
-  let f  := fun t => ⟦ FormalSum.mul' R G s t ⟧ 
+  let f  := fun t => ⟦ FormalSum.mul R G s t ⟧ 
   apply  Quotient.lift f
   apply func_eql_of_move_equiv
-  intro t t' rel
+  intro t t rel
   simp 
   induction rel with
   | zeroCoeff tail g a hyp =>
     rw [hyp]
     apply Quotient.sound
-    simp [mul']
+    simp [mul]
     apply funext
     intro x₀
     rw [← append_coords]
-    let l := mulTerm_zero' R G g x₀ s
+    let l := mulTerm_zero R G g x₀ s
     rw [l]
     simp [zero_add]
   | addCoeffs a b x tail =>
     apply Quotient.sound
     apply funext; intro x₀
-    simp [mul']
+    simp [mul]
     repeat (rw [← append_coords])
     admit
     
   | cons a x s₁ s₂ r step =>
     apply Quotient.sound
     apply funext ; intro x₀
-    simp [mul']
+    simp [mul]
     rw [← append_coords]
     rw [← append_coords]
     simp 
     let l := Quotient.exact step
-    let l' := congrFun l x₀
+    let l := congrFun l x₀
     rw [l]
   | swap a₁ a₂ x₁ x₂ tail =>
     apply Quotient.sound
     apply funext ; intro x₀
-    simp [mul', ← append_coords]
+    simp [mul, ← append_coords]
     rw [← add_assoc]
     rw [← add_assoc]
     simp
     let lc := 
       add_comm 
-        (coords (mulTerm' R G a₁ x₁ s) x₀)
-        (coords (mulTerm' R G a₂ x₂ s) x₀)
+        (coords (mulTerm R G a₁ x₁ s) x₀)
+        (coords (mulTerm R G a₂ x₂ s) x₀)
     rw [lc] 
-
-end flipped
